tez.v
@@ -4,12 +4,12 @@ Require Import ZArith.
 Require int64.
 Require Eqdep_dec.
 
-Definition tez : Set := {t : int64.int64 | int64.sign t = false }.
+Definition mutez : Set := {t : int64.int64 | int64.sign t = false }.
 
-Definition to_int64 (t : tez) : int64.int64 :=
+Definition to_int64 (t : mutez) : int64.int64 :=
   let (t, _) := t in t.
 
-Definition to_int64_inj (t1 t2 : tez) :
+Definition to_int64_inj (t1 t2 : mutez) :
   to_int64 t1 = to_int64 t2 -> t1 = t2.
 Proof.
   intro H.
@@ -23,23 +23,23 @@ Proof.
   destruct (Bool.bool_dec x y); tauto.
 Qed.
 
-Coercion to_int64 : tez >-> int64.int64.
+Coercion to_int64 : mutez >-> int64.int64.
 
-Definition to_Z (t : tez) : Z := int64.to_Z t.
+Definition to_Z (t : mutez) : Z := int64.to_Z t.
 
-Definition of_int64 (t : int64.int64) : option tez :=
-  match int64.sign t as b return int64.sign t = b -> option tez with
+Definition of_int64 (t : int64.int64) : option mutez :=
+  match int64.sign t as b return int64.sign t = b -> option mutez with
   | false => fun H => Some (exist _ t H)
   | true => fun _ => None
   end eq_refl.
 
-Definition of_Z (t : Z) : option tez :=
+Definition of_Z (t : Z) : option mutez :=
   of_int64 (int64.of_Z t).
 
-Definition compare (t1 t2 : tez) : comparison :=
+Definition compare (t1 t2 : mutez) : comparison :=
   int64.compare (to_int64 t1) (to_int64 t2).
 
-Lemma compare_eq_iff (t1 t2 : tez) : compare t1 t2 = Eq <-> t1 = t2.
+Lemma compare_eq_iff (t1 t2 : mutez) : compare t1 t2 = Eq <-> t1 = t2.
 Proof.
   unfold compare.
   rewrite int64.compare_eq_iff.
